src/Specific/ReificationTypes.v
@@ -1,0 +1,201 @@
+Require Import Coq.ZArith.ZArith.
+Require Import Coq.romega.ROmega.
+Require Import Coq.micromega.Lia.
+Require Import Coq.Lists.List.
+Local Open Scope Z_scope.
+
+Require Import Crypto.Arithmetic.Core.
+Require Import Crypto.Arithmetic.PrimeFieldTheorems.
+Require Import Crypto.Util.FixedWordSizes.
+Require Import Crypto.Util.Tuple.
+Require Import Crypto.Util.ZRange Crypto.Util.BoundedWord.
+Require Import Crypto.Util.Tactics.DestructHead.
+Require Import Crypto.Util.Decidable.
+
+Require Import Crypto.Util.Tactics.PoseTermWithName.
+Require Import Crypto.Util.Tactics.CacheTerm.
+
+Ltac pose_limb_widths wt sz limb_widths :=
+  pose_term_with
+    ltac:(fun _ => (eval vm_compute in (List.map (fun i => Z.log2 (wt (S i) / wt i)) (seq 0 sz))))
+           limb_widths.
+
+Ltac get_b_of upper_bound_of_exponent :=
+  constr:(fun exp => {| lower := 0 ; upper := upper_bound_of_exponent exp |}%Z). (* max is [(0, 2^(exp+2) + 2^exp + 2^(exp-1) + 2^(exp-3) + 2^(exp-4) + 2^(exp-5) + 2^(exp-6) + 2^(exp-10) + 2^(exp-12) + 2^(exp-13) + 2^(exp-14) + 2^(exp-15) + 2^(exp-17) + 2^(exp-23) + 2^(exp-24))%Z] *)
+
+(* The definition [bounds_exp] is a tuple-version of the limb-widths,
+   which are the [exp] argument in [b_of] above, i.e., the approximate
+   base-2 exponent of the bounds on the limb in that position. *)
+Ltac pose_bounds_exp sz limb_widths bounds_exp :=
+  pose_term_with_type
+    (Tuple.tuple Z sz)
+    ltac:(fun _ => eval compute in
+               (Tuple.from_list sz limb_widths eq_refl))
+           bounds_exp.
+
+Ltac pose_bounds sz b_of bounds_exp bounds :=
+  pose_term_with_type
+    (Tuple.tuple zrange sz)
+    ltac:(fun _ => eval compute in
+               (Tuple.map (fun e => b_of e) bounds_exp))
+           bounds.
+
+Ltac pose_lgbitwidth limb_widths lgbitwidth :=
+  pose_term_with
+    ltac:(fun _ => eval compute in (Z.to_nat (Z.log2_up (List.fold_right Z.max 0 limb_widths))))
+           lgbitwidth.
+
+Ltac pose_bitwidth lgbitwidth bitwidth :=
+  pose_term_with
+    ltac:(fun _ => eval compute in (2^lgbitwidth)%nat)
+           bitwidth.
+
+Ltac pose_feZ sz feZ :=
+  pose_term_with
+    ltac:(fun _ => constr:(tuple Z sz))
+           feZ.
+
+Ltac pose_feW sz lgbitwidth feW :=
+  cache_term_with_type_by
+    Type
+    ltac:(let v := eval cbv [lgbitwidth] in (tuple (wordT lgbitwidth) sz) in exact v)
+           feW.
+Ltac pose_feW_bounded feW bounds feW_bounded :=
+  cache_term_with_type_by
+    (feW -> Prop)
+    ltac:(let v := eval cbv [bounds] in (fun w : feW => is_bounded_by None bounds (map wordToZ w)) in exact_no_check v)
+           feW_bounded.
+Ltac pose_feBW sz bitwidth bounds feBW :=
+  cache_term_with_type_by
+    Type
+    ltac:(let v := eval cbv [bitwidth bounds] in (BoundedWord sz bitwidth bounds) in exact v)
+           feBW.
+
+Lemma feBW_bounded_helper'
+      sz bitwidth bounds
+      (feBW := BoundedWord sz bitwidth bounds)
+      (wt : nat -> Z)
+      (Hwt : forall i, 0 <= wt i)
+  : forall (a : feBW),
+    B.Positional.eval wt (map lower bounds)
+    <= B.Positional.eval wt (BoundedWordToZ sz bitwidth bounds a)
+    <= B.Positional.eval wt (map upper bounds).
+Proof.
+  let a := fresh "a" in
+  intro a;
+    destruct a as [a H]; unfold BoundedWordToZ, proj1_sig.
+  destruct sz as [|sz].
+  { cbv -[Z.le Z.lt Z.mul]; lia. }
+  { cbn [tuple map] in *.
+    revert dependent wt; induction sz as [|sz IHsz]; intros.
+    { cbv -[Z.le Z.lt wordToZ Z.mul Z.pow Z.add lower upper Nat.log2 wordT] in *.
+      repeat match goal with
+             | [ |- context[@wordToZ ?n ?x] ]
+               => generalize dependent (@wordToZ n x); intros
+             | [ H : forall j, 0 <= wt j |- context[wt ?i] ]
+               => pose proof (H i); generalize dependent (wt i); intros
+             end.
+      nia. }
+    { pose proof (Hwt 0%nat).
+      cbn [tuple' map'] in *.
+      destruct a as [a' a], bounds as [bounds b], H as [H [H' _]].
+      cbn [fst snd] in *.
+      setoid_rewrite (@B.Positional.eval_step (S _)).
+      specialize (IHsz bounds a' H (fun i => wt (S i)) (fun i => Hwt _)).
+      nia. } }
+Qed.
+Lemma feBW_bounded_helper
+      sz bitwidth bounds
+      (feBW := BoundedWord sz bitwidth bounds)
+      (wt : nat -> Z)
+      (Hwt : forall i, 0 <= wt i)
+      l u
+  : l <= B.Positional.eval wt (map lower bounds)
+    /\ B.Positional.eval wt (map upper bounds) < u
+    -> forall (a : feBW),
+      l <= B.Positional.eval wt (BoundedWordToZ sz bitwidth bounds a) < u.
+Proof.
+  intros [Hl Hu] a; split;
+    [ eapply Z.le_trans | eapply Z.le_lt_trans ];
+    [ | eapply feBW_bounded_helper' | eapply feBW_bounded_helper' | ];
+    assumption.
+Qed.
+
+Ltac pose_feBW_bounded wt sz feBW bitwidth bounds m wt_nonneg feBW_bounded :=
+  cache_proof_with_type_by
+    (forall a : feBW, 0 <= B.Positional.eval wt (BoundedWordToZ sz bitwidth bounds a) < 2 * Z.pos m)
+    ltac:(apply (@feBW_bounded_helper sz bitwidth bounds wt wt_nonneg);
+          vm_compute; clear; split; congruence)
+           feBW_bounded.
+
+Ltac pose_phiW feW m wt phiW :=
+  cache_term_with_type_by
+    (feW -> F m)
+    ltac:(exact (fun x : feW => B.Positional.Fdecode wt (Tuple.map wordToZ x)))
+           phiW.
+Ltac pose_phiBW feBW m wt phiBW :=
+  cache_term_with_type_by
+    (feBW -> F m)
+    ltac:(exact (fun x : feBW => B.Positional.Fdecode wt (BoundedWordToZ _ _ _ x)))
+           phiBW.
+
+Ltac get_ReificationTypes_package wt sz bounds m wt_nonneg upper_bound_of_exponent :=
+  let limb_widths := fresh "limb_widths" in
+  let bounds_exp := fresh "bounds_exp" in
+  let bounds := fresh "bounds" in
+  let lgbitwidth := fresh "lgbitwidth" in
+  let bitwidth := fresh "bitwidth" in
+  let feZ := fresh "feZ" in
+  let feW := fresh "feW" in
+  let feW_bounded := fresh "feW_bounded" in
+  let feBW := fresh "feBW" in
+  let feBW_bounded := fresh "feBW_bounded" in
+  let phiW := fresh "phiW" in
+  let phiBW := fresh "phiBW" in
+  let limb_widths := pose_limb_widths wt sz limb_widths in
+  let b_of := get_b_of upper_bound_of_exponent in
+  let bounds_exp := pose_bounds_exp sz limb_widths bounds_exp in
+  let bounds := pose_bounds sz b_of bounds_exp bounds in
+  let lgbitwidth := pose_lgbitwidth limb_widths lgbitwidth in
+  let bitwidth := pose_bitwidth lgbitwidth bitwidth in
+  let feZ := pose_feZ sz feZ in
+  let feW := pose_feW sz lgbitwidth feW in
+  let feW_bounded := pose_feW_bounded feW bounds feW_bounded in
+  let feBW := pose_feBW sz bitwidth bounds feBW in
+  let feBW_bounded := pose_feBW_bounded wt sz feBW bitwidth bounds m wt_nonneg feBW_bounded in
+  let phiW := pose_phiW feW m wt phiW in
+  let phiBW := pose_phiBW feBW m wt phiBW in
+  constr:((feZ, feW, feW_bounded, feBW, feBW_bounded, phiW, phiBW)).
+Ltac make_ReificationTypes_package wt sz bounds m wt_nonneg upper_bound_of_exponent :=
+  lazymatch goal with
+  | [ |- { T : _ & T } ] => eexists
+  | [ |- _ ] => idtac
+  end;
+  let pkg := get_ReificationTypes_package wt sz bounds m wt_nonneg upper_bound_of_exponent in
+  exact pkg.
+
+Module Type ReificationTypesPrePackage.
+  Parameter ReificationTypes_package' : { T : _ & T }.
+  Parameter ReificationTypes_package : projT1 ReificationTypes_package'.
+End ReificationTypesPrePackage.
+
+Module MakeReificationTypes (RP : ReificationTypesPrePackage).
+  Definition ReificationTypes_package := RP.ReificationTypes_package.
+  Ltac reduce_proj x :=
+    let RP_ReificationTypes_package := (eval cbv [ReificationTypes_package] in ReificationTypes_package) in
+    let v := (eval cbv [ReificationTypes_package RP_ReificationTypes_package] in x) in
+    exact v.
+  (**
+<<
+terms = 'feZ, feW, feW_bounded, feBW, feBW_bounded, phiW, phiBW'
+for i in terms.split(', '):
+    print("  Notation %s := (ltac:(reduce_proj (let '(%s) := ReificationTypes_package in %s))) (only parsing)." % (i, terms, i))
+>> *)
+  Notation feZ := (ltac:(reduce_proj (let '(feZ, feW, feW_bounded, feBW, feBW_bounded, phiW, phiBW) := ReificationTypes_package in feZ))) (only parsing).
+  Notation feW := (ltac:(reduce_proj (let '(feZ, feW, feW_bounded, feBW, feBW_bounded, phiW, phiBW) := ReificationTypes_package in feW))) (only parsing).
+  Notation feW_bounded := (ltac:(reduce_proj (let '(feZ, feW, feW_bounded, feBW, feBW_bounded, phiW, phiBW) := ReificationTypes_package in feW_bounded))) (only parsing).
+  Notation feBW := (ltac:(reduce_proj (let '(feZ, feW, feW_bounded, feBW, feBW_bounded, phiW, phiBW) := ReificationTypes_package in feBW))) (only parsing).
+  Notation feBW_bounded := (ltac:(reduce_proj (let '(feZ, feW, feW_bounded, feBW, feBW_bounded, phiW, phiBW) := ReificationTypes_package in feBW_bounded))) (only parsing).
+  Notation phiW := (ltac:(reduce_proj (let '(feZ, feW, feW_bounded, feBW, feBW_bounded, phiW, phiBW) := ReificationTypes_package in phiW))) (only parsing).
+  Notation phiBW := (ltac:(reduce_proj (let '(feZ, feW, feW_bounded, feBW, feBW_bounded, phiW, phiBW) := ReificationTypes_package in phiBW))) (only parsing).
+End MakeReificationTypes.
